snake.v
@@ -6,34 +6,6 @@ Require Import Setoid.
 
 Require Import AbGroup.
 
-(* The trivial group *)
-
-Inductive Gr0_set := G0 : Gr0_set.
-
-Theorem Gr0_add_0_l : ∀ x, (λ _ _ : Gr0_set, G0) G0 x = x.
-Proof.
-now intros x; destruct x.
-Qed.
-
-Definition Gr0 :=
-   {| gr_set := Gr0_set;
-      gr_mem _ := True;
-      gr_eq := eq;
-      gr_zero := G0;
-      gr_add _ _ := G0;
-      gr_inv x := x;
-      gr_zero_mem := I;
-      gr_add_mem _ _ _ _ := I;
-      gr_add_0_l := Gr0_add_0_l;
-      gr_add_assoc _ _ _ := eq_refl G0;
-      gr_inv_mem _ H := H;
-      gr_add_inv_r _ := eq_refl;
-      gr_add_comm _ _ := eq_refl G0;
-      gr_equiv := eq_equivalence;
-      gr_mem_compat _ _ _ _ := I;
-      gr_add_compat _ _ _ _ _ _ := eq_refl;
-      gr_inv_compat _ _ H := H |}.
-
 (* Cokernels
 
    x ∈ Coker f ↔ x ∈ H/Im f
